compiler/src/compiler/ExprImpEventLoopSpec.v
@@ -32,20 +32,20 @@ Section Params1.
   Local Set Warnings "-cannot-define-projection".
 
   Record ProgramSatisfiesSpec(init_f loop_f: String.string)
-         (e: env)
+         (e: list (String.string * (list String.string * list String.string * Syntax.cmd)))
          (spec: ProgramSpec): Prop :=
   {
-    funs_valid: ExprImp.valid_funs e;
+    funs_valid: valid_src_funs e = true;
     init_code: Syntax.cmd.cmd;
-    get_init_code: map.get e init_f = Some (nil, nil, init_code);
+    get_init_code: map.get (map.of_list e) init_f = Some (nil, nil, init_code);
     init_code_correct: forall m0 mc0,
         mem_available spec.(datamem_start) spec.(datamem_pastend) m0 ->
-        Semantics.exec e init_code nil m0 map.empty mc0 (hl_inv spec);
+        Semantics.exec (map.of_list e) init_code nil m0 map.empty mc0 (hl_inv spec);
     loop_body: Syntax.cmd.cmd;
-    get_loop_body: map.get e loop_f = Some (nil, nil, loop_body);
+    get_loop_body: map.get (map.of_list e) loop_f = Some (nil, nil, loop_body);
     loop_body_correct: forall t m l mc,
         hl_inv spec t m l mc ->
-        Semantics.exec e loop_body t m l mc (hl_inv spec);
+        Semantics.exec (map.of_list e) loop_body t m l mc (hl_inv spec);
   }.
 
 End Params1.
