end2end/src/end2end/End2EndPipeline.v
@@ -300,12 +300,12 @@ Section Connect.
                    WeakestPrecondition.cmd funspecs loop_body t m l bedrock2Inv) ->
     (* Assumptions on the compiler level: *)
     forall (instrs: list Instruction) positions (required_stack_space: Z),
-    compile_prog compile_ext_call ml (map.of_list funimplsList) = Success (instrs, positions, required_stack_space) ->
+    compile_prog compile_ext_call ml funimplsList = Success (instrs, positions, required_stack_space) ->
     required_stack_space <= word.unsigned (word.sub (stack_pastend ml) (stack_start ml)) / bytes_per_word ->
     word.unsigned (code_start ml) + Z.of_nat (Datatypes.length (instrencode instrs)) <=
       word.unsigned (code_pastend ml) ->
     Forall (fun i : Instruction => verify i iset) instrs ->
-    ExprImp.valid_funs (map.of_list funimplsList) ->
+    valid_src_funs funimplsList = true ->
     (* Assumptions on the Kami level: *)
     kami_mem_contains_bytes (instrencode instrs) ml.(code_start) memInit ->
     forall (t: Kami.Semantics.LabelSeqT) (mFinal: KamiImplMachine),
@@ -352,7 +352,7 @@ Section Connect.
       intros.
       eapply P2establish.
       unfold initial_conditions.
-      exists (map.of_list funimplsList), instrs, positions, required_stack_space.
+      exists funimplsList, instrs, positions, required_stack_space.
       destr_RiscvMachine m0RV.
       subst.
       ssplit.
